CoqOfRust/revm/revm_interpreter/instructions/simulations/arithmetic.v
@@ -1,8 +1,89 @@
 Require Import CoqOfRust.CoqOfRust.
 Require Import CoqOfRust.links.M.
 Require Import CoqOfRust.simulations.M.
-Import simulations.M.Notations.
-Require Import revm.links.dependencies.
+Require Import revm.revm_interpreter.links.interpreter.
+Require Import revm.revm_interpreter.links.interpreter_types.
+Require Import revm.revm_interpreter.simulations.gas.
+Require Import revm.revm_interpreter.simulations.interpreter_types.
+Require Import revm.revm_interpreter.instructions.links.arithmetic.
+
+Import Impl_Gas.
+
+Instance run_add Stack
+    {WIRE H : Set} `{Link WIRE} `{Link H}
+    {WIRE_types : InterpreterTypes.Types.t} `{InterpreterTypes.Types.AreLinks WIRE_types}
+    `(run_InterpreterTypes_for_WIRE : InterpreterTypes.Run WIRE WIRE_types)
+    (interpreter : Ref.t Pointer.Kind.MutRef (Interpreter.t WIRE WIRE_types))
+    (_host : Ref.t Pointer.Kind.MutRef H) :
+  Run.Trait Stack (links.arithmetic.run_add _ interpreter _host).
+Proof.
+  constructor.
+  destruct run_InterpreterTypes_for_WIRE.
+  destruct run_StackTrait_for_Stack, run_LoopControl_for_Control.
+  (* destruct popn_top as [? []].
+  destruct gas as [? []].
+  destruct set_instruction_result as [? []]. *)
+  Time simulate.
+  { Time simulate_destruct; simulate.
+    match goal with
+    | H : _ |- Run.Trait ?Stack (_ ?x1 ?x2) =>
+      apply (H Stack x1 x2)
+    end.
+  }
+    progress cbn in *.
+    idtac.
+    (* destruct link; cbn in *.
+    destruct run_StackTrait_for_Stack, run_LoopControl_for_Control; cbn in *. *)
+    generalize set_instruction_result; clear; intros.
+    match goal with
+    | |- Run.Trait _ (?f _ _) =>
+      set (f' := f) in |- *
+    end.
+    destruct WIRE_types; cbn in *.
+    destruct link, run_LoopControl_for_Control, set_instruction_result0; cbn in *.
+    progress fold f' in set_instruction_result.
+    unfold InterpreterTypes.Types.IsLinkControl in *; cbn in *.
+    with_strategy transparent [Φ φ] apply set_instruction_result.
+    progress fold f' in set_instruction_result.
+    apply set_instruction_result.
+    match goal with
+    | H : forall _ _ _, ?f _ _ _ = _ |- _ =>
+      specialize (H _ _ _ eq_refl)
+    end.
+    Check set_instruction_result.
+    refine (set_instruction_result _ _ _).
+    best.
+    match goal with.
+    dependent apply set_instruction_result.
+    epose proof (set_instruction_result Stack
+      (* ((Ref.cast_to Pointer.Kind.MutRef
+      {|
+        Ref.core :=
+          SubPointer.Runner.apply interpreter.(Ref.core)
+            Interpreter.get_control
+      |})) *)
+      (* instruction_result.InstructionResult.OutOfGas *)
+    ).
+    apply H5.
+    apply set_instruction_result.
+    typeclasses eauto.
+    match goal with
+    | |- context[if ?condition then _ else _] =>
+      let condition' := eval cbv in condition in
+      change condition with condition'
+    end.
+    Time match goal with
+    | |- context[if ?condition then _ else _] =>
+      destruct condition
+    end.
+    { Show.
+    simulate_reduce.
+
+  }
+  4: { intros. apply Impl_Gas.run_record_cost.
+    cbn in output.
+    Show.
+
 (*
 Require Import revm.interpreter.links.interpreter.
 Require Import revm.interpreter.interpreter.links.instruction_result.
