CoqOfRust/revm/revm_interpreter/simulations/interpreter_types.v
@@ -1,0 +1,65 @@
+Require Import CoqOfRust.CoqOfRust.
+Require Import CoqOfRust.links.M.
+Require Import CoqOfRust.simulations.M.
+Require Import revm.revm_interpreter.links.instruction_result.
+Require Import revm.revm_interpreter.links.interpreter_types.
+
+Module StackTrait.
+  Record Run (Self : Set) `{Link Self} (link : StackTrait.Run Self) : Set := {
+    len Stack self :
+      Run.Trait Stack (link.(StackTrait.len).(TraitMethod.run) self);
+    is_empty Stack self :
+      Run.Trait Stack (link.(StackTrait.is_empty).(TraitMethod.run) self);
+    push Stack self value :
+      Run.Trait Stack (link.(StackTrait.push).(TraitMethod.run) self value);
+    push_b256 Stack self value :
+      Run.Trait Stack (link.(StackTrait.push_b256).(TraitMethod.run) self value);
+    popn Stack N self :
+      Run.Trait Stack (link.(StackTrait.popn).(TraitMethod.run) N self);
+    popn_top Stack POPN self :
+      Run.Trait Stack (link.(StackTrait.popn_top).(TraitMethod.run) POPN self);
+    top Stack self :
+      Run.Trait Stack (link.(StackTrait.top).(TraitMethod.run) self);
+    pop Stack self :
+      Run.Trait Stack (link.(StackTrait.pop).(TraitMethod.run) self);
+    pop_address Stack self :
+      Run.Trait Stack (link.(StackTrait.pop_address).(TraitMethod.run) self);
+    exchange Stack self n m :
+      Run.Trait Stack (link.(StackTrait.exchange).(TraitMethod.run) self n m);
+    dup Stack self n :
+      Run.Trait Stack (link.(StackTrait.dup).(TraitMethod.run) self n);
+  }.
+End StackTrait.
+
+Module LoopControl.
+  Record Run (Self : Set) `{Link Self} (link : LoopControl.Run Self) : Set := {
+    set_instruction_result Stack self result :
+      Run.Trait Stack (link.(LoopControl.set_instruction_result).(TraitMethod.run) self result);
+    set_next_action Stack self action result :
+      Run.Trait Stack (link.(LoopControl.set_next_action).(TraitMethod.run) self action result);
+    gas Stack self :
+      Run.Trait Stack (link.(LoopControl.gas).(TraitMethod.run) self);
+    instruction_result Stack self :
+      Run.Trait Stack (link.(LoopControl.instruction_result).(TraitMethod.run) self);
+    take_next_action Stack self :
+      Run.Trait Stack (link.(LoopControl.take_next_action).(TraitMethod.run) self);
+  }.
+End LoopControl.
+
+Module InterpreterTypes.
+  Class Run
+      (Self : Set) `{Link Self}
+      (types : InterpreterTypes.Types.t) `{InterpreterTypes.Types.AreLinks types}
+      (link : InterpreterTypes.Run Self types) :
+      Set :=
+  {
+    run_StackTrait_for_Stack :
+      StackTrait.Run
+        types.(InterpreterTypes.Types.Stack)
+        link.(InterpreterTypes.run_StackTrait_for_Stack);
+    run_LoopControl_for_Control :
+      LoopControl.Run
+        types.(InterpreterTypes.Types.Control)
+        link.(InterpreterTypes.run_LoopControl_for_Control);
+  }.
+End InterpreterTypes.
